src/CP.v
@@ -7,28 +7,13 @@ Section t.
 
   Variable Phi : state.   
   Variable Var : type -> Type.
-
-  Inductive toption A : type -> Type :=
-  | SNone : forall t, toption A t
-  | SSome : forall (b: A), toption A Core.Tbool. 
-
-  Arguments SNone {A} t. 
-  Arguments SSome {A} b. 
-
-  Definition bind {A B t} (F: A -> toption B Tbool) (o: toption A t) : toption B t :=
-    match o with
-        | SNone t => SNone t
-        | SSome x => (F x) end. 
-
-  Notation "'do' X <- A ; B" := 
-  (bind (fun X => B) A)
-    (at level 200, X ident, A at level 100, B at level 200). 
-
-  (* Maybe we have a pointer *)
-  Definition sval := toption BDD.expr. 
-
-  Notation V := (fun t => Var t * sval t)%type.   
   
+  (* Maybe we have a pointer *)
+  Definition sval := option BDD.expr. 
+
+  Notation V := (fun t => Var t * sval)%type.   
+  
+  (* The symbolic values *)
   Inductive bexpr :=
   | Lift : BDD.expr  -> bexpr
   | Ite : forall (c l r : BDD.expr), bexpr
@@ -36,26 +21,23 @@ Section t.
   | Or : forall (a b : BDD.expr), bexpr
   | Xor : forall (a b : BDD.expr), bexpr
   | Not : forall (a : BDD.expr), bexpr.
-  
-  (* Maybe we have a boolean expression *)
-  Definition bexpro := toption bexpr.   
-  
+    
   (* bang := lift Lift *)
-  Notation bang := (bind (fun x => SSome (Lift x))). 
-  Notation "!!" := (SNone _). 
+  Notation bang x := (do e <- x; (Some (Lift e))). 
+  Notation "!!" := (None). 
 
   Notation bop op dl:= 
   (let a := DList.hd dl in 
    let b := DList.hd (DList.tl dl) in 
-     do a <- (snd a);
-     do b <- (snd b);
-     SSome (op a b)). 
+     do a <- (snd a);            (* take the symbolic value of a *)
+     do b <- (snd b);            (* take the symbolic value of b *)
+     Some (op a b)).            (* apply the operation on the symbolic values *)
 
   Require Import RTL. 
-  Definition cp_expr t (e : expr Phi V t) : (expr Phi Var t) * (toption bexpr t). 
+  Definition cp_expr t (e : expr Phi V t) : (expr Phi Var t) * (option bexpr). 
   refine (match e with
             | Evar t x => 
-                match t as ty return V ty -> (expr Phi Var ty) * (toption bexpr ty) with 
+                match t as ty return V ty -> (expr Phi Var ty) * (option bexpr) with 
                   | Tbool => fun y => (Evar (fst y), bang (snd y)) 
                   | t => fun y  => (Evar (fst y), !!) end x
             | Eread t v => (Eread v, !!)
@@ -63,35 +45,35 @@ Section t.
             | Ebuiltin tys res f args  => 
                 (Ebuiltin f (DList.map (fun _ x => fst x) args), _)           
             | Econstant t x => 
-                match t as ty return constant ty -> (expr Phi Var ty * toption bexpr ty) with
+                match t as ty return constant ty -> (expr Phi Var ty * option bexpr) with
                   | Tbool => fun c => if ( c : bool)
-                                    then (Econstant c, SSome (Lift BDD.T))
-                                    else (Econstant c, SSome (Lift BDD.F))
+                                    then (Econstant c, Some (Lift BDD.T))
+                                    else (Econstant c, Some (Lift BDD.F))
                   | t => fun c => (Econstant c, !!) end x
             | Emux ty c l r => 
                 (_ ,
-                 match ty as t return V t -> V t  -> toption bexpr t with 
+                 match ty as t return V t -> V t  -> option bexpr with 
                    | Tbool => fun l r =>  
                                (do c <- (snd c);
                                 do l <- (snd l);
                                 do r <- (snd r);
-                                SSome (Ite c l r))
+                                Some (Ite c l r))
                    | _ => fun _ _ => !! end l r)
             | Efst l t v => (Efst (fst v) , !!)
             | Esnd l t v => (Esnd (fst v) , !!)
             | Enth l t m v => (Enth m (fst v), !!)
             | Etuple l dl => (Etuple (DList.map (fun _ x => fst x) dl), !!)
           end). 
-  refine (match f in builtin tys res return DList.T V tys -> toption bexpr res with
+  refine (match f in builtin tys res return DList.T V tys -> option bexpr with
             | BI_andb => fun dl =>  bop And dl
             | BI_orb  => fun dl =>  bop Or  dl
             | BI_xorb => fun dl =>  bop Xor dl
-            | BI_negb => fun dl =>  do e <- (snd (DList.hd dl)); SSome (Not e)
+            | BI_negb => fun dl =>  do e <- (snd (DList.hd dl)); Some (Not e)
             | _ => fun _ => !!
           end args); simpl.
   refine (match snd c with 
-                   | SSome BDD.T => (Evar (fst l))
-                   | SSome BDD.F => (Evar (fst r))
+                   | Some BDD.T => (Evar (fst l))
+                   | Some BDD.F => (Evar (fst r))
                    |  _ => Emux (fst c) (fst l) (fst r) end).  
   Defined. 
 
@@ -102,25 +84,25 @@ Section t.
       Enext: nat
     }. 
 
-  Definition empty : Env := mk BDD.empty [] 100. 
+  Definition empty : Env := mk BDD.empty [] 20. 
   
   Definition add_bdd (Gamma: Env) (b:bexpr ): option (BDD.expr * Env) :=  
     match b with
       | Lift x => Some (x, Gamma)
       | Ite c l r => 
-          do r, bdd <- BDD.ite (Ebdd Gamma) c l r;
-          Some (r, mk bdd (Eknown Gamma) (Enext Gamma))
+          do v, bdd <- BDD.ite (Ebdd Gamma) (Enext Gamma) c l r;
+          Some (v, mk bdd (Eknown Gamma) (Enext Gamma))
       | And a b => 
-          do  r,bdd <- BDD.andb (Ebdd Gamma) a b;
+          do  r,bdd <- BDD.andb (Ebdd Gamma) (Enext Gamma) a b;
           Some (r, mk bdd (Eknown Gamma) (Enext Gamma))
       | Or a b => 
-          do  r,bdd <- BDD.orb (Ebdd Gamma) a b;
+          do  r,bdd <- BDD.orb (Ebdd Gamma) (Enext Gamma) a b;
           Some (r, mk bdd (Eknown Gamma) (Enext Gamma))
       | Xor a b => 
-          do r,bdd  <- BDD.xorb (Ebdd Gamma) a b;
+          do r,bdd  <- BDD.xorb (Ebdd Gamma) (Enext Gamma) a b;
           Some (r, mk bdd (Eknown Gamma) (Enext Gamma))
       | Not a => 
-          do r,bdd <- BDD.negb (Ebdd Gamma) a;
+          do r,bdd <- BDD.negb (Ebdd Gamma) (Enext Gamma) a;
           Some (r, mk bdd (Eknown Gamma) (Enext Gamma))
     end. 
 
@@ -140,54 +122,46 @@ Section t.
     match T with
       | & x => & x
       | telescope_bind arg b cont => 
-          let (e,svo) := cp_expr arg b in 
-            match svo in toption _ arg return 
-               (Var arg * sval arg -> telescope Phi V A) -> 
-               expr Phi Var arg -> telescope Phi Var A 
-            with 
-              | @SNone  arg => 
-                  match arg as ty return 
-                     (Var ty * sval ty -> telescope Phi V A) -> 
-                     expr Phi Var ty -> telescope Phi Var A 
-                  with 
-                    | Tbool => fun cont e => 
-                                (
-                                  k :- e; 
-                                  let (ptr, Gamma) := incr Gamma in 
-                                    let Gamma := add_env Gamma k ptr in
-                                      cp_telescope Gamma (cont (k, SSome ptr)))
-                    | _ => fun cont e => 
-                            k :- e; cp_telescope Gamma (cont (k, SNone _))
+        let (e,sv) := cp_expr arg b in 
+        match arg return 
+              (Var arg * sval -> telescope Phi V A) -> 
+              expr Phi Var arg -> telescope Phi Var A 
+        with 
+          | Tbool => 
+            match sv with 
+              | None => 
+                fun cont e => 
+                  (
+                    k :- e; 
+                    let (ptr, Gamma) := incr Gamma in 
+                    let Gamma := add_env Gamma k ptr in (* we add the mapping ptr ~> k in the environment *)
+                    cp_telescope Gamma (cont (k, Some ptr))
+                  )
+              | Some v => 
+                fun cont e =>  
+                  match add_bdd Gamma v with 
+                    | Some (ptr, Gamma) =>
+                      (* the symbolic value correspond to a pointer in the bdd *)
+                      match lookup Gamma ptr with
+                        | None => (* this pointer does not correspond to a
+                                 value. We bind this value, and add it
+                                 to the environment*)                          
+                          (k :- e;
+                           let Gamma := add_env Gamma k ptr in 
+                           cp_telescope  Gamma (cont (k, Some ptr)))
+                        | Some old => 
+                          (* This pointer was already mapped to a value. No need to bind a new value *)
+                          cp_telescope Gamma (cont (old, (Some ptr))) 
+                      end
+                    | None => 
+                      (* adding to the bdd failed. This should not happen, but is safe *)
+                      k :- e; cp_telescope Gamma (cont (k,None))
                   end
-              | SSome sv => 
-                  (* We have a symbolic value *)
-                  fun cont e =>  
-                    match add_bdd Gamma sv with 
-                      | Some (ptr, Gamma) =>
-                          (* the symbolic value correspond to a pointer in the bdd *)
-                          match lookup Gamma ptr with
-                            | None =>
-                                (* this pointer does not
-                                          correspond to a value. We
-                                          bind this value, and add it
-                                          to the environment*)
-                                k :- e;
-                                let Gamma := add_env Gamma k ptr in 
-                                  cp_telescope Gamma (cont (k, SSome ptr))
-                            | Some old => 
-                                (* the pointer was already
-                                          associated. No need to bind
-                                          a new value *)
-                                cp_telescope Gamma (cont (old, (SSome ptr))) 
-                          end
-                      | None => 
-                          (* adding to the bdd failed. This
-                                    should not happen, but is safe *)
-                          k :- e; cp_telescope Gamma (cont (k,SNone _))
-                    end
-            end cont e
-    end. 
-
+            end
+          | _ => fun cont e => 
+                  k :- e; cp_telescope Gamma (cont (k, None))
+        end cont e
+    end.  
 
   Definition cp_effects (eff: effects Phi V) : effects Phi Var :=
     DList.map
@@ -205,14 +179,342 @@ Section t.
   
   
   Definition cp_block  t (b : block Phi V t) : block Phi Var t :=    
-    let b := ( _ :- @Econstant  _ _ Tbool true ;
-               _ :- @Econstant  _ _ Tbool false ;
-               b) in 
+    (* let b := ( _ :- @Econstant  _ _ Tbool true ; *)
+    (*            _ :- @Econstant  _ _ Tbool false ; *)
+    (*            b) in  *)
     k :-- cp_telescope empty b;
     match k with (v,g,e) =>
                    & (fst v, fst g, cp_effects  e)
     end. 
-End t. 
+End t.   
+
+Notation V := (fun t => eval_type t * sval)%type.   
+
+Definition lift (env : list (BDD.expr * bool)) : BDD.var -> bool :=
+  fun n => 
+    match List.nth_error env n with 
+      | None => true
+      | Some (e,b) => b
+    end. 
+
+
+Definition interp (E: Env eval_type) v := 
+  BDD.interp (lift (Eknown _ E)) (Ebdd _ E) (S (Enext _ E)) v. 
+
+
+Definition eval_bexpr (E: Env eval_type) (b: bexpr) : option (bool) :=
+  match b with
+    | Lift x => interp E x 
+    | Ite c l r => do c <- interp E c; 
+                  do l <- interp E l;
+                  do r <- interp E r;
+                  Some (if c then l else r)
+    | And a b => do a <- interp E a; 
+                do b <- interp E b; 
+                Some (a && b)%bool
+    | Or a b => do a <- interp E a; 
+               do b <- interp E b; 
+               Some (a || b)%bool
+    | Xor a b => do a <- interp E a; 
+                do b <- interp E b; 
+                Some (xorb a b)%bool
+    | Not a => do a <- interp E a; 
+              Some (negb a)%bool
+  end. 
+
+Notation "G |= x -- y" := (In _ _ _ x y G) (no associativity, at level 71). 
+
+Definition value (E: Env eval_type) sv x := match sv with 
+                                                None => False
+                                              | Some v => BDD.value (lift (Eknown _ E)) (Ebdd _ E) v x
+                                            end. 
+
+
+  
+Class inv (G: Gamma eval_type V) (E: Env eval_type) :=
+  {
+    inv_1 : forall t (x : eval_type t) y, G |= x -- y -> x = fst y;
+    inv_2 : forall (x: eval_type Tbool) y, G |= x -- y -> 
+                                      value E (snd y) x; 
+    inv_bdd_wf : BDD.wf (lift  (Eknown _ E)) (Ebdd _ E); 
+    inv_next : (Enext _ E) = BDD.wf_depth _ _ inv_bdd_wf
+  }. 
+    
+Lemma inv_interp {G E} {Hinv : inv G E} (x: eval_type Tbool) y e:
+  forall (H: G |= x -- (y, Some e)),  
+    interp E e = Some x. 
+Proof. 
+  intros. 
+  unfold interp. 
+  rewrite inv_next. apply BDD.interp_S.  apply BDD.wf_value_interp.  
+  apply inv_2 in H. simpl in H. apply H. 
+Qed. 
+ 
+Notation R := (fun G t x y => In _ _ t x y G).  
+
+(** The dependent type swiss-knife. *)
+Ltac t :=  subst; repeat match goal with 
+                       H : existT _ _ _ = existT _ _ _ |- _ => 
+                         apply Eqdep.EqdepTheory.inj_pair2 in H
+                   |   H : context [eq_rect ?t _ ?x ?t ?eq_refl] |- _ => 
+                         rewrite <- Eqdep.EqdepTheory.eq_rect_eq in H
+                   |   H : context [eq_rect ?t _ ?x ?t ?H'] |- _ => 
+                         rewrite (Eqdep.EqdepTheory.UIP_refl _ _ H') in H;
+                         rewrite <- Eqdep.EqdepTheory.eq_rect_eq in H
+                   |   H : existT _ ?t1 ?x1 = existT _ ?t2 ?x2 |- _ => 
+                         let H' := fresh "H'" in 
+                           apply EqdepFacts.eq_sigT_sig_eq in H; destruct H as [H H']; subst
+                         end; subst.
+
+(* Lemma Gamma_inv_cons_bool G env e f sv :  *)
+(*   Gamma_inv G env -> *)
+(*   value env sv e ->  *)
+(*   forall (heq: e = f),  *)
+(*     Gamma_inv (cons eval_type V Tbool e (f,sv) G) env.  *)
+(* Proof.  *)
+(*   intros. constructor.  *)
+(*   - intros. inversion H0; t. reflexivity. apply Gamma_inv_1. eauto.  *)
+(*   - intros. admit.  *)
+(* Qed.  *)
+
+(* Lemma Gamma_inv_cons G env t e f:  *)
+(*   Gamma_inv G env -> *)
+(*   t <> Tbool ->  *)
+(*   forall  Heq : e = f,  *)
+(*     Gamma_inv (cons eval_type V t e (f,None) G) env.  *)
+(* Proof.  *)
+(*   intros. constructor.  *)
+(*   - intros. inversion H0; t. reflexivity. apply Gamma_inv_1. eauto.  *)
+(*   - intros. admit.  *)
+(* Qed.         *)
+
+Lemma cp_expr_correct Phi st : 
+  forall t e1 r1, 
+    eval_expr Phi st t e1 = r1 ->
+    forall G (env : Env eval_type) e2,
+      expr_equiv _ _ Phi (R G) t e1 e2 ->     
+      inv G env
+      -> match t as ty return eval_type ty -> Prop
+        with 
+          | Tbool => 
+            match snd (cp_expr Phi _ t  e2) 
+            with
+              | Some sv => fun r1 => eval_bexpr env sv  = Some r1
+              | None => fun _ => True
+            end
+          | _ => fun _ => True
+        end r1.
+Proof. 
+  destruct 1; inversion 1; t;  try solve [destruct t; simpl; auto]; intros. 
+  - simpl. destruct t; trivial; clear H. 
+    Require Import Equality. 
+
+    Ltac d :=
+      repeat match goal with 
+        | H : DList.pointwise _ (?t :: ?q) _ _ |- _ => 
+          apply DList.inversion_pointwise in H; 
+            destruct H
+        | H : DList.pointwise _  [] _ _ |- _ => clear H
+        | x :( _ * sval)%type |- _ => destruct x as [ ? [? | ]]
+      end. 
+
+    dependent destruction f; simpl; repeat DList.inversion; d; simpl; trivial;  
+    repeat match goal with 
+      | H :    ?G |= ?x -- (?v, Some ?e) |- context [?e] => 
+        rewrite (inv_interp _ _ _ H)
+    end; simpl; try reflexivity. 
+  - destruct t; trivial. destruct c; reflexivity.   
+  - destruct t; trivial; d;  simpl; trivial.  
+    repeat match goal with 
+             | H :    ?G |= ?x -- (?v, Some ?e) |- context [?e] => 
+               rewrite (inv_interp _ _ _ H)
+           end; simpl; try reflexivity. 
+  - trivial. 
+  - trivial. 
+Qed. 
+
+
+Lemma cp_effects_correct (Phi : state) st Delta G e  (Hg : inv G e):
+  forall e1 e2 
+  (H : effects_equiv eval_type V Phi (RTL.R eval_type V G) e1 e2), 
+   eval_effects Phi st e1 Delta =
+   eval_effects Phi st (cp_effects Phi eval_type e2) Delta. 
+Proof. 
+  intros e1 e2 H.
+  apply DList.map3_map.   
+  eapply DList.pointwise_map; [| apply H];
+  clear H; simpl in *; intros. 
+  inversion H;  t; unfold RTL.R in *; 
+  repeat (match goal with 
+            | |- ?x = ?x  => reflexivity
+            | |- context [match ?x with _=> _ end] => 
+              case_eq x; intros
+            | H' : In _ _ _ ?x ?y _ |- _ => 
+              rewrite (inv_1 _ _ _ H')
+            | H : context [fst ?x] |- _ => progress (simpl in H)
+            | H : ?x = ?x |- _ => clear H
+            | H : ?y = ?x, H' : ?x = ?y |- _ => clear H'
+            | x : (_ * _)%type |- _ =>  destruct x; simpl; subst
+          end); simpl. 
+Qed. 
+Lemma inv_cons_None G E t e f: 
+  inv G E -> 
+  e = f -> 
+  inv (cons eval_type V t e (f, None) G) E. 
+Proof. 
+  intros Hinv Heq; subst. 
+  econstructor. 
+  + intros.  
+    inversion H; t.  reflexivity. 
+    apply Hinv; auto. 
+    
+  + intros. admit. 
+  + apply Hinv. 
+Qed. 
+
+Lemma cp_expr_correct_2 Phi st G env (Hg : inv G env) t:
+  forall e1 e2, expr_equiv eval_type V Phi (RTL.R eval_type V G) t e1 e2 ->
+           forall svo e, cp_expr Phi eval_type t e2 = (e,svo) ->
+                           eval_expr Phi st t e1 = eval_expr Phi st t e. 
+Proof.
+  Ltac crush :=
+    repeat (match goal with 
+      | H: (_,_) = (_,_) |- _ => injection H; clear H; intros; subst
+      | Hg : inv _ _ ,  H : In _ _ _ ?x ?y _ |- context [?x] =>
+        rewrite (inv_1 _ _ _ H)
+      | H : DList.T [] |- _ => DList.inversion 
+      | H : DList.T (_ :: _) |- _  => DList.inversion 
+      | H : DList.pointwise _ ( _ :: _) _ _ |- _ => apply DList.inversion_pointwise in H; destruct H
+    end); try reflexivity; try f_equal. 
+  intros e1. destruct e1; intros e2 H; inversion H; t; simpl; intros; unfold RTL.R in *; crush.
+  
+  - simpl. f_equal. 
+    clear H b. 
+    induction args; repeat DList.inversion;simpl; intuition. 
+    + crush.  eauto.  
+  -  destruct ty; crush. destruct c; crush. 
+  - clear H.  
+    destruct c2. simpl.  destruct s; simpl. destruct e3; simpl.
+    
+    Ltac save :=
+      repeat match goal with 
+        |  H : _ |= _ -- _ |- _ =>
+           pose proof (inv_1 _ _ _ H);
+           pose proof (inv_interp _ _ _ H);
+                    clear H
+      end. 
+    save. simpl in *; subst. compute in H0. injection H0; intros; subst. reflexivity. 
+    save. simpl in *; subst. compute in H0. injection H0; intros; subst. reflexivity.
+    reflexivity. 
+    reflexivity. 
+  - simpl. clear H. 
+    induction l; repeat DList.inversion;simpl; intuition. 
+    + crush; eauto. 
+
+Qed. 
+
+
+Lemma cp_telescope_correct (Phi: state) st t  Delta: 
+     forall (b : RTL.block Phi eval_type t)
+       (b': RTL.block Phi V t)
+       (G : Gamma eval_type V),
+       block_equiv eval_type V Phi t G b b' ->
+       forall e,
+       inv  G e
+     ->
+   eval_telescope Phi st
+     (fun x : eval_type t * bool * effects Phi eval_type =>
+      let (y, e0) := x in
+      let (p, g) := y in check g; Some (p, eval_effects Phi st e0 Delta)) b =
+   eval_telescope Phi st
+     (fun x : eval_type t * bool * effects Phi eval_type =>
+      let (y, e0) := x in
+      let (p, g) := y in check g; Some (p, eval_effects Phi st e0 Delta))
+     (k :-- cp_telescope Phi eval_type e b';
+      (let (p, e0) := k in
+       let (v, g) := p in & (fst v, fst g, cp_effects Phi eval_type e0))). 
+Proof. 
+  Ltac crush ::=
+    repeat match goal with 
+             | H: (_,_) = (_,_) |- _ => injection H; clear H; intros; subst
+             | H : In _ _ _ ?x ?y _ |- context [?x] =>
+               rewrite (inv_1 _ _ _ H)
+             | H : DList.T [] |- _ => DList.inversion 
+             | H : DList.T (_ :: _) |- _  => DList.inversion 
+             | H : DList.pointwise _ ( _ :: _) _ _ |- _ => apply DList.inversion_pointwise in H; destruct H
+             | |- Some _ = Some _ => f_equal
+             | |- (_,_) = (_,_) => f_equal
+             | |- context [eval_type _] => simpl eval_type
+           end; try reflexivity. 
+  
+  induction 1 as [G v1 v2 g1 g2 e1 e2 Hv Hg He| G a e1 e2 k1 k2 He Hk IH]; simpl; intros E INV. 
+  - crush.
+    match goal with 
+      |- context [(if ?x then _ else _) = (if ?y then _ else _)] => 
+      let H := fresh in 
+      assert (H : x = y)  by reflexivity; 
+      subst; clear H; destruct x
+    end; f_equal; f_equal. eapply cp_effects_correct; eauto.   
+  - destruct (cp_expr Phi eval_type a e2) as [binding [sv | ]]eqn: Heq; destruct a; 
+    try (apply IH; apply inv_cons_None; eauto using cp_expr_correct_2 ).
+    
+    {
+       destruct (add_bdd eval_type E sv) as [[ptr E2] | ]eqn:Heq2; [|apply IH]. 
+       destruct (lookup eval_type E2 ptr) as [old | ] eqn:Heq3; apply IH.
+       clear IH. 
+       pose proof (cp_expr_correct_2 _ st _ _ INV _ _ _ He _ _ Heq). 
+       rewrite H. 
+       pose proof (cp_expr_correct _ _ _ _ _ H _ _ _ He INV). simpl in H0.
+       rewrite Heq in H0. simpl in H0. 
+       Lemma inv_cons_lookup_Some G E (INV : inv G E) E2 sv ptr old X:
+         add_bdd eval_type E sv = Some (ptr, E2) -> 
+         lookup eval_type E2 ptr = Some old -> 
+         eval_bexpr E sv = Some X -> 
+         inv (cons eval_type V B X (old, Some ptr) G) E2. 
+       Proof. 
+       Admitted. 
+       eapply inv_cons_lookup_Some; eauto. 
+       pose proof (cp_expr_correct_2 _ st _ _ INV _ _ _ He _ _ Heq). 
+       rewrite H. 
+       pose proof (cp_expr_correct _ _ _ _ _ H _ _ _ He INV). simpl in H0.
+       rewrite Heq in H0. simpl in H0.
+       Lemma inv_cons_lookup_None G E (INV : inv G E) E2 sv ptr X:
+         add_bdd eval_type E sv = Some (ptr, E2) -> 
+         lookup eval_type E2 ptr = None -> 
+         eval_bexpr E sv = Some X -> 
+         inv (cons eval_type V B X (X, Some ptr) G) (add_env eval_type E2 X ptr). 
+       Proof. 
+       Admitted. 
+       eapply inv_cons_lookup_None; eauto. 
+       apply inv_cons_None; eauto using cp_expr_correct_2. 
+    }
+    {
+      destruct (incr eval_type E) as [ptr E'] eqn: Hincr.
+      apply IH; clear IH. 
+      eapply cp_expr_correct_2 in Heq; eauto.  
+      rewrite Heq; clear Heq.  
+      generalize (eval_expr Phi st B binding). 
+      intros e. 
+      Lemma inv_cons_incr G E (INV : inv G E) e ptr E2: 
+        incr eval_type E = (ptr, E2) -> 
+        inv (cons eval_type V B e (e, Some ptr) G) (add_env eval_type E2 e ptr).
+      Proof. 
+      Admitted. 
+      eapply inv_cons_incr; eauto. 
+    }
+Qed.     
+
+Lemma Gamma_inv_empty : inv  (nil _ _ ) (empty eval_type). 
+Proof. 
+Admitted. 
+
+Theorem cp_correct Phi st t (b : Block Phi t) Delta : WF Phi t b -> 
+  eval_block Phi st t (b _) Delta = eval_block Phi st t (cp_block Phi eval_type t (b _)) Delta. 
+Proof. 
+  intros.
+  eapply cp_telescope_correct; eauto using Gamma_inv_empty.
+Qed. 
+  
 
 Definition Compile Phi t (b : Block Phi t) : Block Phi t :=  
   fun V => cp_block Phi V t (b _). 
@@ -220,4 +522,7 @@ Definition Compile Phi t (b : Block Phi t) : Block Phi t :=
 Theorem Compile_correct Phi t b (Hwf : WF Phi t b): forall st Delta,
   Eval Phi st t (Compile Phi t b) Delta =  Eval Phi st t b Delta. 
 Proof. 
-Admitted. 
+  unfold Eval. intros. unfold Compile. symmetry. apply cp_correct. auto. 
+Qed. 
+
+Print Assumptions Compile_correct. 
