examples/Driver.v
@@ -1,4 +1,4 @@
 Require Isa Add.
 
 Definition example1 := Isa.t. 
-Definition example2 := (Compiler.copt _ _  (Add.test 3)).
+Definition example2 := (Compiler.copt _ _  (Add.test 2)).
